

MORAWETZ ON MINKOWSKI

ONYX GAUTAM

We compute the deformation tensor of X for a vector field $X = f(r)\partial_r$, then compute the corresponding divergence term K^X .

1. CURRENT FORMALISM

Let φ be a function. The energy-momentum tensor is a symmetric $(0, 2)$ -tensor defined by

$$T_{\alpha\beta}[\varphi] = \partial_\alpha \varphi \partial_\beta \varphi - \frac{1}{2} g_{\alpha\beta} |\nabla \varphi|^2, \quad (1)$$

where we write $|\nabla \varphi|^2 = \nabla^\mu \varphi \nabla_\mu \varphi = g^{\mu\nu} \nabla_\mu \varphi \nabla_\nu \varphi$. This tensor satisfies $\nabla^\alpha T_{\alpha\beta} = \square \varphi \nabla_\beta \varphi$, so the energy momentum tensor associated to the solution of the wave equation is divergence free. For a vector field X , we introduce the associated current (a one-form)

$$J_\alpha^X[\varphi] = T_{\alpha\beta}[\varphi] X^\beta \quad (2)$$

and the deformation tensor

$${}^{(X)}\pi_{\alpha\beta} = \frac{1}{2} (\mathcal{L}_X g)_{\alpha\beta} = \frac{1}{2} (\nabla_\alpha X_\beta + \nabla_\beta X_\alpha). \quad (3)$$

The divergence of the one-form J^X satisfies

$$\nabla^\alpha J_\alpha^X[\varphi] = K^X[\varphi] + \mathcal{E}^X[\varphi]. \quad (4)$$

where

$$K^X[\varphi] = {}^{(X)}\pi^{\alpha\beta} T_{\alpha\beta}[\varphi] = {}^{(X)}\pi(d\varphi, d\varphi) - \frac{1}{2} \text{tr} {}^{(X)}\pi |\nabla \varphi|^2 \quad (5)$$

and

$$\mathcal{E}^X := X\varphi \square \varphi. \quad (6)$$

Moreover, if w is a weight function, we introduce the auxiliary current

$$J_\alpha^{\text{aux}, w}[\varphi] = w\varphi \nabla_\alpha \varphi - \frac{1}{2} \varphi^2 \nabla_\alpha w. \quad (7)$$

The divergence of this one form is given by

$$\nabla^\alpha J_\alpha^{\text{aux}, w}[\varphi] = K^{\text{aux}, w}[\varphi] + \mathcal{E}^{\text{aux}, w}[\varphi] \quad (8)$$

for

$$K^{\text{aux}, w}[\varphi] := w |\nabla \varphi|^2 - \frac{1}{2} \square w \varphi^2 \quad (9)$$

and

$$\mathcal{E}^{\text{aux}, w}[\varphi] := w\varphi \square \varphi \quad (10)$$

Notice that

$$K^X[\varphi] + K^{\text{aux}, w}[\varphi] = {}^{(X)}\pi(d\varphi, d\varphi) + \left(w - \frac{1}{2} \text{tr} {}^{(X)}\pi\right) |\nabla \varphi|^2 - \frac{1}{2} \square w \varphi^2. \quad (11)$$

2. DEFORMATION TENSOR COMPUTATIONS

Recall that the Minkowski metric in polar coordinates is

$$g = -dt^2 + dr^2 + \mathcal{g}, \quad (12)$$

where $\mathcal{g} = r^2 g_{\mathbf{S}^2}$ for $g_{\mathbf{S}^2}$ the round metric on the unit sphere.

Lemma 2.1. *Let Y be a vector field and set $X = f(r)Y$. Then*

$${}^{(X)}\pi_{\alpha\beta} = f {}^{(Y)}\pi_{\alpha\beta} + \frac{1}{2}(\nabla_\alpha f Y_\beta + \nabla_\beta f Y_\alpha). \quad (13)$$

and

$$\mathrm{tr} {}^{(X)}\pi = f \mathrm{tr} {}^{(Y)}\pi + Yf. \quad (14)$$

If Y is a coordinate vector field, then

$${}^{(Y)}\pi_{\alpha\beta} = \frac{1}{2}Y g_{\alpha\beta}. \quad (15)$$

Proof. Using $X = fY$, compute

$${}^{(X)}\pi_{\alpha\beta} = f {}^{(Y)}\pi_{\alpha\beta} + \frac{1}{2}(\nabla_\alpha f Y_\beta + \nabla_\beta f Y_\alpha). \quad (16)$$

From (13) we obtain

$$\mathrm{tr} {}^{(X)}\pi = f \mathrm{tr} {}^{(Y)}\pi + Yf. \quad (17)$$

Using the definition ${}^{(Y)}\pi = \frac{1}{2}\mathcal{L}_Y g$, we compute (assuming Y is a coordinate vector field so that $\mathcal{L}_Y \partial_\alpha = 0$)

$$2 {}^{(Y)}\pi_{\alpha\beta} = (\mathcal{L}_Y g)(\partial_\alpha, \partial_\beta) = Yg(\partial_\alpha, \partial_\beta) - g(\mathcal{L}_Y \partial_\alpha, \partial_\beta) - g(\partial_\alpha, \mathcal{L}_Y \partial_\beta) = Yg_{\alpha\beta} \quad (18)$$

□

Lemma 2.2. *Write $Y = \partial_r$ and set $X = f(r)\partial_r = f(r)Y$. Write $f' = \partial_r f$. We have*

$$\mathrm{tr} {}^{(X)}\pi = \frac{2}{r}f + f'. \quad (19)$$

and

$${}^{(X)}\pi(d\varphi, d\varphi) = f'(\partial\varphi)^2 + \frac{f}{r}|\nabla\varphi|^2. \quad (20)$$

Proof. Using (15) and the diagonal form of the metric, compute that the non-zero components of ${}^{(Y)}\pi$ are

$${}^{(Y)}\pi_{ab} = \frac{1}{r}\mathcal{g}_{ab}. \quad (21)$$

It follows immediately that

$$\mathrm{tr} {}^{(Y)}\pi = \frac{2}{r} \quad (22)$$

and hence

$$\mathrm{tr} {}^{(X)}\pi = \frac{2}{r}f + f'. \quad (23)$$

Since the only non-zero component of Y with down indices is $Y_r = g_{rr}Y^r = g_{rr} = 1$, and f is a function only of r , the second term in (13) contributes only when $\alpha = \beta = r$. It follows that

$${}^{(X)}\pi_{rr} = f' \quad {}^{(X)}\pi_{ab} = \frac{f}{r}\mathcal{g}_{ab}. \quad (24)$$

We now compute

$${}^{(X)}\pi(d\varphi, d\varphi) = f'(\partial_r\varphi)^2 + \frac{f}{r}|\nabla\varphi|^2. \quad (25)$$

□

3. COMPUTING THE BULK DIVERGENCE TERM

Define

$$K^f[\varphi] := K^{f(r)\partial_r}[\varphi] + K^{\text{aux}, r^{-1}f(r)}[\varphi]. \quad (26)$$

Lemma 3.1. *We have*

$$K^f[\varphi] = \frac{1}{2}f'[(\partial_t\varphi)^2 + (\partial_r\varphi)^2] + \left(\frac{f}{r} - \frac{f'}{2}\right)|\nabla\varphi|^2 - \frac{1}{2}r^{-1}f''\varphi^2. \quad (27)$$

Proof. From (11) and lemma 2.2, we have

$$K^X[\varphi] + K^{\text{aux}, w}[\varphi] = f'(\partial_r\varphi)^2 + \frac{f}{r}|\nabla\varphi|^2 + \left(w - \frac{f}{r} - \frac{1}{2}f'\right)|\nabla\varphi|^2 - \frac{1}{2}\square w\varphi^2. \quad (28)$$

Take $w = r^{-1}f$. To obtain the desired result, compute

$$\square w = r^{-2}\partial_r(r^2\partial_r(r^{-1}f)) = r^{-1}f'' \quad (29)$$

and recall that $|\nabla\varphi|^2 = -(\partial_t\varphi)^2 + (\partial_r\varphi)^2 + |\nabla\varphi|^2$. □